vaddm etc. in steel; vevictbm left

steel/Veritas.Steel.Verifier.fst
@@ -26,7 +26,111 @@ let prf_update_hash p r t thread_id = sladmit()
 
 let update_clock (ts:T.timestamp) (vs:thread_state_t) = sladmit()
 
-#push-options "--query_stats --log_queries --fuel 0 --ifuel 1"
+//Needs an unfold, else weirdness
+unfold
+let slot_ok (s:U16.t) (vs:_) (h:rmem (thread_state_inv vs))
+  = U16.v s < length (v_thread vs h).model_store
+
+assume
+val points_to_some_slot (s:U16.t)
+                        (d:bool)
+                        (vs:_)
+  : Steel bool
+    (thread_state_inv vs)
+    (fun _ -> thread_state_inv vs)
+    (requires fun h -> True) //U16.v s < length (v_thread vs h).model_store)
+    (ensures fun h0 b h1 ->
+      U16.v s < length (v_thread vs h0).model_store /\
+      b == VerifierModel.points_to_some_slot (v_thread vs h0) s d /\
+      v_thread vs h0 == v_thread vs h1)
+
+assume
+val madd_to_store (s:U16.t) (k:T.key) (v:T.value) (s':U16.t) (d:bool)
+                  (vs:_)
+  : Steel unit
+    (thread_state_inv vs)
+    (fun _ -> thread_state_inv vs)
+    (requires fun h0 ->
+      slot_ok s vs h0 /\
+      slot_ok s' vs h0)
+    (ensures fun h0 _ h1 ->
+      slot_ok s vs h0 /\
+      slot_ok s' vs h0 /\
+      v_thread vs h1 == model_madd_to_store (v_thread vs h0) s k v s' d)
+
+assume
+val madd_to_store_split (s:U16.t) (k:T.key) (v:T.value) (s':U16.t) (d d':bool)
+                        (vs:_)
+  : Steel unit
+    (thread_state_inv vs)
+    (fun _ -> thread_state_inv vs)
+    (requires fun h0 ->
+      slot_ok s vs h0 /\
+      slot_ok s' vs h0)
+    (ensures fun h0 _ h1 ->
+      slot_ok s vs h0 /\
+      slot_ok s' vs h0 /\
+      v_thread vs h1 == model_madd_to_store_split (v_thread vs h0) s k v s' d d')
+
+assume
+val vevictb_update_hash_clock
+       (s:U16.t)
+       (t:T.timestamp)
+       (vs:_)
+   : Steel unit
+     (thread_state_inv vs)
+     (fun _ -> thread_state_inv vs)
+     (requires fun h0 ->
+       U16.v s < length (v_thread vs h0).model_store /\
+       VerifierModel.sat_evictb_checks (v_thread vs h0) s t)
+     (ensures fun h0 _ h1 ->
+       U16.v s < length (v_thread vs h0).model_store /\
+       VerifierModel.sat_evictb_checks (v_thread vs h0) s t /\
+       v_thread vs h1 ==
+       model_vevictb_update_hash_clock (v_thread vs h0) s t)
+
+assume
+val bevict_from_store (s:U16.t) (vs:_)
+  : Steel unit
+    (thread_state_inv vs)
+    (fun _ -> thread_state_inv vs)
+    (requires fun h0 ->
+       U16.v s < length (v_thread vs h0).model_store)
+    (ensures fun h0 _ h1 ->
+       U16.v s < length (v_thread vs h0).model_store /\
+       v_thread vs h1 ==
+       model_bevict_from_store (v_thread vs h0) s)
+
+assume
+val update_value (s:U16.t) (v:T.value) (vs:_)
+  : Steel unit
+    (thread_state_inv vs)
+    (fun _ -> thread_state_inv vs)
+    (requires fun h0 ->
+      U16.v s  < length (v_thread vs h0).model_store /\
+      has_slot (v_thread vs h0) s /\
+      is_value_of (key_of_slot (v_thread vs h0) s) v)
+    (ensures fun h0 _ h1 ->
+      U16.v s  < length (v_thread vs h0).model_store /\
+      has_slot (v_thread vs h0) s /\
+      is_value_of (key_of_slot (v_thread vs h0) s) v /\
+      v_thread vs h1 == model_update_value (v_thread vs h0) s v)
+
+assume
+val mevict_from_store (s s':_) (d:_) (vs:_)
+  : Steel unit
+    (thread_state_inv vs)
+    (fun _ -> thread_state_inv vs)
+    (requires fun h0 ->
+       U16.v s < length (v_thread vs h0).model_store /\
+       U16.v s' < length (v_thread vs h0).model_store)
+    (ensures fun h0 _ h1 ->
+       U16.v s < length (v_thread vs h0).model_store /\
+       U16.v s' < length (v_thread vs h0).model_store /\
+       v_thread vs h1 ==
+       model_mevict_from_store (v_thread vs h0) s s' d)
+
+#push-options "--query_stats --fuel 0 --ifuel 1"
 #restart-solver
 let fail vs msg = write vs.failed true; ()
 
@@ -65,6 +169,151 @@ let vput (s:U16.t) (k:T.key) (v:T.data_value) (vs: thread_state_t)
         ()
       )
 
+val vaddm (s:U16.t) (r:T.record) (s':U16.t) (vs:_)
+  : Steel unit
+    (thread_state_inv vs)
+    (fun _ -> thread_state_inv vs)
+    (requires fun h0 ->
+      U16.v s  < length (v_thread vs h0).model_store /\
+      U16.v s' < length (v_thread vs h0).model_store)
+    (ensures fun h0 _ h1 ->
+      U16.v s  < length (v_thread vs h0).model_store /\
+      U16.v s' < length (v_thread vs h0).model_store /\
+      v_thread vs h1 == vaddm_model (v_thread vs h0) s r s')
+
+let coerce #a #p (x:a) (pf:squash (p x)) : x:a{p x} = x
+
+let vaddm s r s' vs
+  = let h = get () in
+    assert (U16.v s  < length (v_thread vs h).model_store);  //this assert seems necessary
+    let k = r.T.record_key in
+    let v = r.T.record_value in
+    (* check store contains slot s' *)
+    let r' = VCache.vcache_get_record vs.st s' in
+    match r' with
+    | None -> fail vs "Slot missing"
+    | Some r' ->
+      let k' = r'.record_key in
+      let v' = r'.record_value in
+      (* check k is a proper desc of k' *)
+      if not (is_proper_descendent k k') then fail vs "not proper descendent"
+      (* check store does not contain slot s *)
+      else (
+        let r_old = VCache.vcache_get_record vs.st s in
+        if Some? r_old then fail vs "old record exists"
+        else if not (is_value_of k v) then fail vs "incompatible value for key"
+        else let Some v' = to_merkle_value v' in
+             let d = desc_dir k k' in
+             let dh' = desc_hash_dir v' d in
+             let h = hashfn v in
+             match dh' with
+             | T.Dh_vnone _ -> (* k' has no child in direction d *)
+             (* first add must be init value *)
+               if v <> init_value k then fail vs "incorrect initial value"
+               else let b = points_to_some_slot s' d vs in
+                    if b then fail vs "points to some slot"
+                    else (
+                      let tsm = madd_to_store s k v s' d vs in
+                      let v'_upd = update_merkle_value v' d k h false in
+                      update_value s' (T.V_mval v'_upd) vs
+                    )
+
+        | T.Dh_vsome {T.dhd_key=k2; T.dhd_h=h2; T.evicted_to_blum = b2} ->
+          if k2 = k then (* k is a child of k' *)
+            (* check hashes match and k was not evicted to blum *)
+            if not (h2 = h && b2 = T.Vfalse) then fail vs "hash mismatch or evicted"
+            (* check slot s' does not contain a desc along direction d *)
+            else (
+              let b = points_to_some_slot s' d vs in
+              if b then fail vs "points to some slot"
+              else madd_to_store s k v s' d vs
+            )
+          else (
+            (* first add must be init value *)
+            if v <> init_value k then fail vs "not init value"
+            (* check k2 is a proper desc of k *)
+            else
+              let b = (is_proper_descendent k2 k) in
+                if not b
+                then fail vs "not proper descendent"
+                else (
+                  let pf : squash (is_proper_descendent k2 k) = () in
+                  //need this weird coercion to avoid mysterious failures
+                  let k : (k:T.key { is_proper_descendent k2 k }) = coerce k pf in
+                  let d2 = desc_dir k2 k in
+                  let Some mv = to_merkle_value v in
+                  let mv_upd = update_merkle_value mv d2 k2 h2 (b2=T.Vtrue) in
+                  let v'_upd = update_merkle_value v' d k h false in
+                  let b = points_to_some_slot s' d vs in
+                  //can't share the continuation
+                  if b
+                  then (
+                    madd_to_store_split s k (T.V_mval mv_upd) s' d d2 vs;
+                    update_value s' (T.V_mval v'_upd) vs
+                  )
+                  else (
+                    madd_to_store s k (T.V_mval mv_upd) s' d vs;
+                    update_value s' (T.V_mval v'_upd) vs
+                  )
+             )))
+
+val vevictm (s s':U16.t) (vs:_)
+  : Steel unit
+    (thread_state_inv vs)
+    (fun _ -> thread_state_inv vs)
+    (requires fun h0 ->
+      U16.v s  < length (v_thread vs h0).model_store /\
+      U16.v s' < length (v_thread vs h0).model_store)
+    (ensures fun h0 _ h1 ->
+      U16.v s  < length (v_thread vs h0).model_store /\
+      U16.v s' < length (v_thread vs h0).model_store /\
+      v_thread vs h1 == vevictm_model (v_thread vs h0) s s')
+let vevictm s s' vs
+  = let h = get () in
+    assert (U16.v s  < length (v_thread vs h).model_store);  //this assert seems necessary
+    if s = s' then fail vs "Equal slots"
+    else (
+      let r = VCache.vcache_get_record vs.st s in
+      let r' = VCache.vcache_get_record vs.st s' in
+      match r, r' with
+      | None, _
+      | _, None -> fail vs "Empty slots"
+      | Some r, Some r' ->
+        let k = r.record_key in
+        let v = r.record_value in
+        let k' = r'.record_key in
+        let v' = r'.record_value in
+        (* check k is a proper descendent of k' *)
+        if not (is_proper_descendent k k') then fail vs "Not proper descendent"
+        (* check k does not have a (merkle) child in the store *)
+        else
+          let b1 = points_to_some_slot s true vs in
+          let b2 = points_to_some_slot s false vs in
+          if b1 || b2
+          then fail vs "Points to some slot"
+          else (
+            let d = desc_dir k k' in
+            let Some v' = to_merkle_value v' in
+            let dh' = desc_hash_dir v' d in
+            match dh' with
+            | T.Dh_vnone _ -> fail vs "No child"
+            | T.Dh_vsome {T.dhd_key=k2; T.dhd_h=h2; T.evicted_to_blum = b2} ->
+              if k2 <> k then fail vs "k2 <> k"
+              else if Some? r.record_parent_slot &&
+                    (fst (Some?.v r.record_parent_slot) <> s' ||
+                     snd (Some?.v r.record_parent_slot) <> d)
+              then fail vs "parent slot mismatch"
+              else let b = points_to_some_slot s' d vs in
+                   if None? r.record_parent_slot
+                   && b
+                   then fail vs "parent slot mismatch"
+                   else (
+                     let h = hashfn v in //Lower
+                     let v'_upd = update_merkle_value v' d k h false in
+                     let tsm = update_value s' (T.V_mval v'_upd) vs in
+                     mevict_from_store s s' d vs
+                   )
+          ))
 
 let vaddb (s:U16.t)
           (r:T.record)
@@ -100,19 +349,6 @@ let vaddb (s:U16.t)
         VCache.vcache_add_record vs.st s k v T.BAdd)
     )
 
-assume
-val points_to_some_slot (s:U16.t)
-                        (d:bool)
-                        (vs:_)
-  : Steel bool
-    (thread_state_inv vs)
-    (fun _ -> thread_state_inv vs)
-    (requires fun h -> U16.v s < length (v_thread vs h).model_store)
-    (ensures fun h0 b h1 ->
-      U16.v s < length (v_thread vs h0).model_store /\
-      b == VerifierModel.points_to_some_slot (v_thread vs h0) s d /\
-      v_thread vs h0 == v_thread vs h1)
-
 val sat_evictb_checks (s:U16.t)
                       (t:T.timestamp)
                       (vs:_)
@@ -139,35 +375,6 @@ let sat_evictb_checks s t vs
         let b2 = points_to_some_slot s false vs in
         not b1 && not b2
       )
-
-assume
-val vevictb_update_hash_clock
-       (s:U16.t)
-       (t:T.timestamp)
-       (vs:_)
-   : Steel unit
-     (thread_state_inv vs)
-     (fun _ -> thread_state_inv vs)
-     (requires fun h0 ->
-       U16.v s < length (v_thread vs h0).model_store /\
-       VerifierModel.sat_evictb_checks (v_thread vs h0) s t)
-     (ensures fun h0 _ h1 ->
-       U16.v s < length (v_thread vs h0).model_store /\
-       VerifierModel.sat_evictb_checks (v_thread vs h0) s t /\
-       v_thread vs h1 ==
-       model_vevictb_update_hash_clock (v_thread vs h0) s t)
-
-assume
-val bevict_from_store (s:U16.t) (vs:_)
-  : Steel unit
-    (thread_state_inv vs)
-    (fun _ -> thread_state_inv vs)
-    (requires fun h0 ->
-       U16.v s < length (v_thread vs h0).model_store)
-    (ensures fun h0 _ h1 ->
-       U16.v s < length (v_thread vs h0).model_store /\
-       v_thread vs h1 ==
-       model_bevict_from_store (v_thread vs h0) s)
 
 let vevictb (s:U16.t)
             (t:T.timestamp)
